

Exam 2 Practice Solutions

Jordan Hoffart

1. (a) Compute the derivative of $f(x) = \log(x)$ at $x_0 = 1$ with $h = 0.1$ and $h = 0.05$ using

$$f'(x) \approx \frac{f(x+4h) - f(x-2h)}{6h}.$$

Solution. For $h = 0.1$,

$$f'(1) \approx \frac{\log(1.4) - \log(0.8)}{0.6} \approx 0.9326929798923711.$$

For $h = 0.05$,

$$f'(1) \approx \frac{\log(1.2) - \log(0.9)}{0.3} \approx 0.9589402415059362.$$

□

- (b) Derive the error of the method using Taylor expansions.

Solution.

$$f(x+4h) = f(x) + 4hf'(x) + 8h^2f''(\xi_+)$$

for some $\xi_+ \in (x, x+4h)$, and

$$f(x-2h) = f(x) - 2hf'(x) + 2h^2f''(\xi_-)$$

for some $\xi_- \in (x-2h, x)$. Therefore,

$$\frac{f(x+4h) - f(x-2h)}{6h} - f'(x) = \frac{h}{3}(f''(\xi_+) - f''(\xi_-)) + hf''(\xi_+).$$

Using the Mean Value Theorem, there is $\xi \in (\xi_-, \xi_+)$ such that

$$f''(\xi_+) - f''(\xi_-) = f'''(\xi)(\xi_+ - \xi_-).$$

Thus, since $\xi_+ - \xi_- \leq x+4h - (x-2h) = 6h$,

$$\left| \frac{f(x+4h) - f(x-2h)}{6h} - f'(x) \right| \leq 2h^2 \max_{\xi \in [x-2h, x+4h]} |f'''(\xi)| + h \max_{\xi \in [x, x+4h]} |f''(\xi)|.$$

For $f(x) = \log(x)$,

$$\left| \frac{f(x+4h) - f(x-2h)}{6h} - f'(x) \right| \leq \frac{4h^2}{(x-2h)^3} + \frac{h}{x^2} = \mathcal{O}\left(\frac{h}{x^2}\right).$$

□

2. Approximate

$$\int_{-3}^3 x^2 - x \, dx$$

by using Lagrange interpolation with quadrature points $x = -2$ and $x = 2$.

Solution. Let $f(x) = x^2 - x$, let $x_0 = -2$, $x_1 = 2$, and let

$$L_0(x) = \frac{x - x_1}{x_0 - x_1} = -\frac{x - 2}{4},$$

$$L_1(x) = \frac{x - x_0}{x_1 - x_0} = \frac{x + 2}{4},$$

$$p(x) = f(x_0)L_0(x) + f(x_1)L_1(x) = -6\frac{x - 2}{4} + 2\frac{x + 2}{4}.$$

Then,

$$\begin{aligned} \int_{-3}^3 x^2 - x \, dx &\approx \int_{-3}^3 p(x) \, dx = f(x_0) \int_{-3}^3 L_0(x) \, dx + f(x_1) \int_{-3}^3 L_1(x) \, dx \\ &= 6 \cdot 3 + 2 \cdot 3 = 24. \end{aligned}$$

□

3. Find the coefficients a, b, c, d such that

$$\int_{-1}^1 f(x) dx \approx af(-1) + bf(0) + cf'(-1) + df'(0)$$

has degree of precision 3.

Solution. Using the monomial basis $f(x) = 1, f(x) = x, f(x) = x^2, f(x) = x^3$,

$$2 = a + b,$$

$$0 = -a + c + d,$$

$$2/3 = a - 2c,$$

$$0 = -a + 3c.$$

We solve the last 2 equations for a and c . Adding:

$$2/3 = c.$$

Then, $a = 3c = 2$. Then, from the first equation, $b = 0$, and, from the second equation, $d = a - c = 2 - 2/3 = 4/3$. Thus,

$$a = 2, b = 0, c = 2/3, d = 4/3.$$

□

4. Solve $y' = -2y + 2t$, $y(0) = 0$ using the forward and backward Euler methods with timestep $\Delta t = 0.2$ to final time $T = 1$. Discuss your results.

Solution. Forward Euler:

$$y_{n+1} = y_n + 2(\Delta t)(t_n - y_n).$$

Backward Euler:

$$y_{n+1} = y_n + 2(\Delta t)(t_{n+1} - y_{n+1}).$$

Solving for y_{n+1} :

$$y_{n+1} = \frac{y_n + 2(\Delta t)(t_n + \Delta t)}{1 + 2\Delta t}.$$

Starting with $y_0 = 0$,

FE

0.0	0.00000
0.2	0.00000
0.4	0.08000
0.6	0.20800
0.8	0.36480
1.0	0.53888

BE

0.0	0.00000
0.2	0.05714
0.4	0.15510
0.6	0.28221
0.8	0.43015
1.0	0.59296

The forward Euler solution is always less than the backward Euler solution, and the forward Euler solution always gives 0 as the solution for the first time step. It appears that the backward Euler method is better for this problem with this choice of timestep. \square

5. Consider the following multistep method:

$$w_{i+1} = \frac{1}{2}w_i + \frac{1}{2}w_{i-1} + \frac{h}{2}f(t_i, w_{i+1}) + \frac{h}{2}f(t_i, w_i).$$

(a) Verify that the method is zero-stable.

Solution. The characteristic polynomial for this method is

$$p(\lambda) = \lambda^2 - \frac{1}{2}\lambda - \frac{1}{2}.$$

This has roots

$$\lambda = \frac{1/2 \pm \sqrt{1/4 + 4/2}}{2} = \frac{1}{4} \pm \frac{3}{4} = -\frac{1}{2}, 1.$$

Since all roots have magnitude at most 1, and since the $\lambda = 1$ root has multiplicity 1, the method is strongly zero-stable. \square

(b) Derive the condition on h required for linear stability.

Solution. Inserting $f(t, w) = \lambda w$ with $\lambda < 0$,

$$w_{i+1} = \frac{1}{2}w_i + \frac{1}{2}w_{i-1} + \frac{h}{2}\lambda w_{i+1} + \frac{h}{2}\lambda w_i.$$

Then, moving everything to one side and collecting terms:

$$w_{i+1}(1 - h\lambda/2) - w_i(1 + h\lambda)/2 - 1/2 = 0.$$

The corresponding characteristic polynomial is

$$p(z) = (1 - h\lambda/2)z^2 - (1/2 + h\lambda/2)z - 1/2.$$

Linear stability requires that the roots of this polynomial must be less than 1 in magnitude. Since the roots of p don't change if we multiply by a constant, let's multiply by 2 for convenience and look at the roots of

$$q(z) = (2 - h\lambda)z^2 - (1 + h\lambda)z - 1.$$

The roots are

$$z = \frac{1 + h\lambda \pm \sqrt{(1 + h\lambda)^2 + 4(2 - h\lambda)}}{4 - 2h\lambda}.$$

Thus, the linear stability condition is

$$\left| \frac{1 + h\lambda \pm \sqrt{(1 + h\lambda)^2 + 4(2 - h\lambda)}}{4 - 2h\lambda} \right| < 1.$$

\square